monads: add constant state to nondet monad
Extend the nondet_monad with a reader/environment monad component.

- Constrain the underlying state to an extensible record where "env"
  is the constant state and the record extension is the rest of the
  state.
- Update basic monad operations accordingly
- Add new primitive asks for the constant state
- Update rest of monad lemmas and development accordingly

Signed-off-by: Gerwin Klein <gerwin.klein@proofcraft.systems>

lib/Monads/nondet/Nondet_Empty_Fail.thy
@@ -16,7 +16,7 @@ section \<open>Monads that are wellformed w.r.t. failure\<close>
 text \<open>
   Usually, well-formed monads constructed from the primitives in @{text Nondet_Monad} will have the following
   property: if they return an empty set of results, they will have the failure flag set.\<close>
-definition empty_fail :: "('s,'a) nondet_monad \<Rightarrow> bool" where
+definition empty_fail :: "('c, 's,'a) nondet_monad \<Rightarrow> bool" where
   "empty_fail m \<equiv> \<forall>s. fst (m s) = {} \<longrightarrow> snd (m s)"
 
 text \<open>Useful in forcing otherwise unknown executions to have the @{const empty_fail} property.\<close>
