lib/Monads/nondet/Nondet_Monad.thy
@@ -24,42 +24,71 @@ text \<open>
 
 section "The Monad"
 
+record 'c monad_state_record =
+  env :: 'c
+
+type_synonym ('c, 's) monad_state = "('c, 's) monad_state_record_scheme"
+
+type_synonym ('c, 's) mpred = "('c, 's) monad_state \<Rightarrow> bool"
+
+abbreviation monad_state :: "'c \<Rightarrow> 's \<Rightarrow> ('c, 's) monad_state" where
+  "monad_state c \<equiv> \<lambda>s. \<lparr> env = c, \<dots> = s \<rparr>"
+
+abbreviation mstate :: "('c, 's) monad_state \<Rightarrow> 's" where
+  "mstate \<equiv> monad_state_record.more"
+
+abbreviation with_env_of :: "('c, 's) monad_state \<Rightarrow> 't \<Rightarrow> ('c, 't) monad_state" where
+  "with_env_of s \<equiv> monad_state (env s)"
+
+definition map_state :: "('s \<Rightarrow> 't) \<Rightarrow> ('c, 's) monad_state \<Rightarrow> ('c, 't) monad_state"
+  where
+  "map_state f \<equiv> \<lambda>s. with_env_of s (f (mstate s))"
+
+definition const_env ::
+  "(('c, 's) monad_state \<Rightarrow> ('d, 't) monad_state) \<Rightarrow> ('c, 's) monad_state \<Rightarrow> ('c, 't) monad_state"
+  where
+  "const_env f \<equiv> \<lambda>s. with_env_of s (mstate (f s))"
+
+definition is_const_env :: "(('c, 's) monad_state \<Rightarrow> ('c, 't) monad_state) \<Rightarrow> bool"
+  where
+  "is_const_env f \<equiv> \<forall>s. env (f s) = env s"
+
 text \<open>
   The basic type of the nondeterministic state monad with failure is
   very similar to the normal state monad. Instead of a pair consisting
-  of result and new state, we return a set of these pairs coupled with
-  a failure flag. Each element in the set is a potential result of the
-  computation. The flag is @{const True} if there is an execution path
-  in the computation that may have failed. Conversely, if the flag is
-  @{const False}, none of the computations resulting in the returned
-  set can have failed.\<close>
-type_synonym ('s, 'a) nondet_monad = "'s \<Rightarrow> ('a \<times> 's) set \<times> bool"
-
+  of result @{typ 'a} and new state @{typ 's}, we return a set of these
+  pairs coupled with a failure flag. Each element in the set is a potential
+  result of the computation. The flag is @{const True} if there is an
+  execution path in the computation that may have failed. Conversely, if
+  the flag is @{const False}, none of the computations resulting in the
+  returned set has failed. The monad also takes as input an environment
+  state @{typ 'c}, which is constant throughout the execution.\<close>
+type_synonym ('c, 's, 'a) nondet_monad = "('c, 's) monad_state \<Rightarrow> ('a \<times> 's) set \<times> bool"
 
 text \<open>
-  Print the type @{typ "('s,'a) nondet_monad"} instead of its unwieldy expansion.
+  Print the type @{typ "('c, 's, 'a) nondet_monad"} instead of its unwieldy expansion.
   Needs an AST translation in code, because it needs to check that the state variable
   @{typ 's} occurs twice. This comparison is not guaranteed to always work as expected
   (AST instances might have different decoration), but it does seem to work here.\<close>
 print_ast_translation \<open>
   let
-    fun monad_tr _ [t1, Ast.Appl [Ast.Constant @{type_syntax prod},
+    fun monad_tr _ [Ast.Appl [Ast.Constant @{type_syntax monad_state}, env, st],
+                    Ast.Appl [Ast.Constant @{type_syntax prod},
                           Ast.Appl [Ast.Constant @{type_syntax set},
-                            Ast.Appl [Ast.Constant @{type_syntax prod}, t2, t3]],
+                            Ast.Appl [Ast.Constant @{type_syntax prod}, rv, st']],
                           Ast.Constant @{type_syntax bool}]] =
-      if t3 = t1
-      then Ast.Appl [Ast.Constant @{type_syntax "nondet_monad"}, t1, t2]
+      if st = st'
+      then Ast.Appl [Ast.Constant @{type_syntax "nondet_monad"}, env, st, rv]
       else raise Match
   in [(@{type_syntax "fun"}, monad_tr)] end
 \<close>
-
 
 text \<open>
   The definition of fundamental monad functions @{text return} and
   @{text bind}. The monad function @{text "return x"} does not change
   the  state, does not fail, and returns @{text "x"}.\<close>
-definition return :: "'a \<Rightarrow> ('s,'a) nondet_monad" where
-  "return a \<equiv> \<lambda>s. ({(a,s)},False)"
+definition return :: "'a \<Rightarrow> ('c,'s,'a) nondet_monad" where
+  "return a \<equiv> \<lambda>s. ({(a, mstate s)},False)"
 
 text \<open>
   The monad function @{text "bind f g"}, also written @{text "f >>= g"},
@@ -69,30 +98,46 @@ text \<open>
   the combined operation is the union of the set of sets that is created
   by @{text g} applied to the result sets of @{text f}. The combined
   operation may have failed, if @{text f} may have failed or @{text g} may
-  have failed on any of the results of @{text f}.\<close>
+  have failed on any of the results of @{text f}. The environment passed to
+  @{text g} is the same as the one passed to @{term f}.\<close>
 definition bind ::
-  "('s, 'a) nondet_monad \<Rightarrow> ('a \<Rightarrow> ('s, 'b) nondet_monad) \<Rightarrow> ('s, 'b) nondet_monad" (infixl ">>=" 60)
+  "('c, 's, 'a) nondet_monad \<Rightarrow> ('a \<Rightarrow> ('c, 's, 'b) nondet_monad) \<Rightarrow> ('c, 's, 'b) nondet_monad"
+  (infixl ">>=" 60)
   where
-  "bind f g \<equiv> \<lambda>s. (\<Union>(fst ` case_prod g ` fst (f s)),
-                   True \<in> snd ` case_prod g ` fst (f s) \<or> snd (f s))"
+  "bind f g \<equiv> \<lambda>s. (\<Union>(fst ` case_prod g ` apsnd (with_env_of s) ` fst (f s)),
+                   True \<in> snd ` case_prod g ` apsnd (with_env_of s) ` fst (f s) \<or> snd (f s))"
 
 text \<open>Sometimes it is convenient to write @{text bind} in reverse order.\<close>
 abbreviation (input) bind_rev ::
-  "('c \<Rightarrow> ('a, 'b) nondet_monad) \<Rightarrow> ('a, 'c) nondet_monad \<Rightarrow> ('a, 'b) nondet_monad" (infixl "=<<" 60)
+  "('a \<Rightarrow> ('c, 's, 'b) nondet_monad) \<Rightarrow> ('c, 's, 'a) nondet_monad \<Rightarrow> ('c, 's, 'b) nondet_monad"
+  (infixl "=<<" 60)
   where
   "g =<< f \<equiv> f >>= g"
 
 text \<open>
   The basic accessor functions of the state monad. @{text get} returns
   the current state as result, does not fail, and does not change the state.
-  @{text "put s"} returns nothing (@{typ unit}), changes the current state
-  to @{text s} and does not fail.\<close>
-definition get :: "('s,'s) nondet_monad" where
-  "get \<equiv> \<lambda>s. ({(s,s)}, False)"
+  @{text ask} returns the constant part of the state as result, does not
+  change the state and does not fail. @{text "put s"} returns nothing
+  (@{typ unit}), changes the current state to @{text s} and does not fail.
 
-definition put :: "'s \<Rightarrow> ('s, unit) nondet_monad" where
-  "put s \<equiv> \<lambda>_. ({((),s)}, False)"
+  We choose to return the full state of the monad in @{text get}, including the
+  constant part, because we later want @{text gets} to return the same kind of
+  state that Hoare logic predicates expect, and those will need access to the
+  full state. This means, @{text modify} and @{text put} should both also take
+  the full state as their argument (ignoring the constant part of their
+  argument), to keep the standard @{text get}/@{text put} laws intact. This
+  integrates well with how @{text gets} and @{text modify} are intended to be
+  used with a record type state -- the standard record update and access
+  will expect the full state type, not only the variable part of the state.\<close>
+definition get :: "('c,'s, ('c,'s) monad_state) nondet_monad" where
+  "get \<equiv> \<lambda>s. ({(s, mstate s)}, False)"
 
+definition ask :: "('c,'s,'c) nondet_monad" where
+  "ask \<equiv> \<lambda>s. ({(env s, mstate s)}, False)"
+
+definition put :: "('c,'s) monad_state \<Rightarrow> ('c, 's, unit) nondet_monad" where
+  "put s \<equiv> \<lambda>_. ({((), mstate s)}, False)"
 
 subsection "Nondeterminism"
 
@@ -100,13 +145,13 @@ text \<open>
   Basic nondeterministic functions. @{text "select A"} chooses an element
   of the set @{text A}, does not change the state, and does not fail
   (even if the set is empty). @{text "f \<sqinter> g"} executes @{text f} or
-  executes @{text g}. It retuns the union of results of @{text f} and
+  executes @{text g}. It returns the union of results of @{text f} and
   @{text g}, and may have failed if either may have failed.\<close>
-definition select :: "'a set \<Rightarrow> ('s,'a) nondet_monad" where
-  "select A \<equiv> \<lambda>s. (A \<times> {s}, False)"
+definition select :: "'a set \<Rightarrow> ('c, 's, 'a) nondet_monad" where
+  "select A \<equiv> \<lambda>s. (A \<times> {mstate s}, False)"
 
 definition alternative ::
-  "('s, 'a) nondet_monad \<Rightarrow> ('s, 'a) nondet_monad \<Rightarrow> ('s, 'a) nondet_monad" (infixl "\<sqinter>" 20)
+  "('c, 's, 'a) nondet_monad \<Rightarrow> ('c, 's, 'a) nondet_monad \<Rightarrow> ('c, 's, 'a) nondet_monad" (infixl "\<sqinter>" 20)
   where
   "f \<sqinter> g \<equiv> \<lambda>s. (fst (f s) \<union> fst (g s), snd (f s) \<or> snd (g s))"
 
@@ -115,69 +160,75 @@ text \<open>
   as in normal @{text select}, the second component indicates whether the
   execution failed. This is useful to lift monads between different state
   spaces.\<close>
-definition select_f :: "'a set \<times> bool  \<Rightarrow> ('s,'a) nondet_monad" where
-  "select_f S \<equiv> \<lambda>s. (fst S \<times> {s}, snd S)"
+definition select_f :: "'a set \<times> bool  \<Rightarrow> ('c, 's, 'a) nondet_monad" where
+  "select_f S \<equiv> \<lambda>s. (fst S \<times> {mstate s}, snd S)"
 
 text \<open>
   @{text state_select} takes a relationship between states, and outputs
   nondeterministically a state related to the input state. Fails if no such
   state exists.\<close>
-definition state_select :: "('s \<times> 's) set \<Rightarrow> ('s, unit) nondet_monad" where
-  "state_select r \<equiv> \<lambda>s. ((\<lambda>x. ((), x)) ` {s'. (s, s') \<in> r}, \<not> (\<exists>s'. (s, s') \<in> r))"
-
+definition state_select ::
+  "(('c,'s) monad_state \<times> ('c,'s) monad_state) set \<Rightarrow> ('c, 's, unit) nondet_monad" where
+  "state_select r \<equiv> \<lambda>s. ((\<lambda>x. ((), mstate x)) ` {s'. (s, s') \<in> r}, \<not> (\<exists>s'. (s, s') \<in> r))"
 
 subsection "Failure"
 
 text \<open>
   The monad function that always fails. Returns an empty set of results and sets the failure flag.\<close>
-definition fail :: "('s, 'a) nondet_monad" where
+definition fail :: "('c, 's, 'a) nondet_monad" where
   "fail \<equiv> \<lambda>s. ({}, True)"
 
 text \<open>Assertions: fail if the property @{text P} is not true\<close>
-definition assert :: "bool \<Rightarrow> ('a, unit) nondet_monad" where
+definition assert :: "bool \<Rightarrow> ('c, 's, unit) nondet_monad" where
   "assert P \<equiv> if P then return () else fail"
 
 text \<open>Fail if the value is @{const None}, return result @{text v} for @{term "Some v"}\<close>
-definition assert_opt :: "'a option \<Rightarrow> ('b, 'a) nondet_monad" where
+definition assert_opt :: "'a option \<Rightarrow> ('c, 's, 'a) nondet_monad" where
   "assert_opt v \<equiv> case v of None \<Rightarrow> fail | Some v \<Rightarrow> return v"
 
 text \<open>An assertion that also can introspect the current state.\<close>
-definition state_assert :: "('s \<Rightarrow> bool) \<Rightarrow> ('s, unit) nondet_monad" where
+definition state_assert :: "('c,'s) mpred \<Rightarrow> ('c, 's, unit) nondet_monad" where
   "state_assert P \<equiv> get >>= (\<lambda>s. assert (P s))"
 
 subsection "Generic functions on top of the state monad"
 
 text \<open>Apply a function to the current state and return the result without changing the state.\<close>
-definition gets :: "('s \<Rightarrow> 'a) \<Rightarrow> ('s, 'a) nondet_monad" where
+definition gets :: "(('c,'s) monad_state \<Rightarrow> 'a) \<Rightarrow> ('c, 's, 'a) nondet_monad" where
   "gets f \<equiv> get >>= (\<lambda>s. return (f s))"
 
+text \<open>Apply a function to the constant state and return the result without changing the state.\<close>
+definition asks :: "('c \<Rightarrow> 'a) \<Rightarrow> ('c, 's, 'a) nondet_monad" where
+  "asks f \<equiv> ask >>= (\<lambda>s. return (f s))"
+
 text \<open>Modify the current state using the function passed in.\<close>
-definition modify :: "('s \<Rightarrow> 's) \<Rightarrow> ('s, unit) nondet_monad" where
+definition modify ::
+  "(('c, 's) monad_state \<Rightarrow> ('c, 's) monad_state) \<Rightarrow> ('c, 's, unit) nondet_monad"
+  where
   "modify f \<equiv> get >>= (\<lambda>s. put (f s))"
 
 lemma simpler_gets_def:
-  "gets f = (\<lambda>s. ({(f s, s)}, False))"
+  "gets f = (\<lambda>s. ({(f s, mstate s)}, False))"
   by (simp add: gets_def return_def bind_def get_def)
 
 lemma simpler_modify_def:
-  "modify f = (\<lambda>s. ({((), f s)}, False))"
+  "modify f = (\<lambda>s. ({((), mstate (f s))}, False))"
   by (simp add: modify_def bind_def get_def put_def)
 
 text \<open>Execute the given monad when the condition is true, return @{text "()"} otherwise.\<close>
-definition "when" :: "bool \<Rightarrow> ('s, unit) nondet_monad \<Rightarrow> ('s, unit) nondet_monad" where
+definition "when" :: "bool \<Rightarrow> ('c, 's, unit) nondet_monad \<Rightarrow> ('c, 's, unit) nondet_monad" where
   "when P m \<equiv> if P then m else return ()"
 
 text \<open>Execute the given monad unless the condition is true, return @{text "()"} otherwise.\<close>
-definition unless :: "bool \<Rightarrow> ('s, unit) nondet_monad \<Rightarrow> ('s, unit) nondet_monad" where
+definition unless :: "bool \<Rightarrow> ('c, 's, unit) nondet_monad \<Rightarrow> ('c, 's, unit) nondet_monad" where
   "unless P m \<equiv> when (\<not>P) m"
 
 text \<open>
   Perform a test on the current state, performing the left monad if
   the result is true or the right monad if the result is false. \<close>
 definition condition ::
-  "('s \<Rightarrow> bool) \<Rightarrow> ('s, 'r) nondet_monad \<Rightarrow> ('s, 'r) nondet_monad \<Rightarrow> ('s, 'r) nondet_monad"
+  "('c,'s) mpred \<Rightarrow> ('c, 's, 'r) nondet_monad \<Rightarrow> ('c, 's, 'r) nondet_monad \<Rightarrow> ('c, 's, 'r) nondet_monad"
   where
-  "condition P L R \<equiv> \<lambda>s. if (P s) then (L s) else (R s)"
+  "condition P L R \<equiv> \<lambda>s. if P s then L s else R s"
 
 notation (output)
   condition  ("(condition (_)//  (_)//  (_))" [1000,1000,1000] 1000)
@@ -185,13 +236,15 @@ notation (output)
 text \<open>
   Apply an option valued function to the current state, fail if it returns @{const None},
   return @{text v} if it returns @{term "Some v"}.\<close>
-definition gets_the :: "('s \<Rightarrow> 'a option) \<Rightarrow> ('s, 'a) nondet_monad" where
+definition gets_the :: "(('c,'s) monad_state \<Rightarrow> 'a option) \<Rightarrow> ('c, 's, 'a) nondet_monad" where
   "gets_the f \<equiv> gets f >>= assert_opt"
 
 text \<open>
   Get a map (such as a heap) from the current state and apply an argument to the map.
   Fail if the map returns @{const None}, otherwise return the value.\<close>
-definition gets_map :: "('s \<Rightarrow> 'a \<Rightarrow> 'b option) \<Rightarrow> 'a \<Rightarrow> ('s, 'b) nondet_monad" where
+definition gets_map ::
+  "(('c,'s) monad_state \<Rightarrow> 'a \<Rightarrow> 'b option) \<Rightarrow> 'a \<Rightarrow> ('c, 's, 'b) nondet_monad"
+  where
   "gets_map f p \<equiv> gets f >>= (\<lambda>m. assert_opt (m p))"
 
 
@@ -200,10 +253,14 @@ subsection \<open>The Monad Laws\<close>
 text \<open>An alternative definition of @{term bind}, sometimes more convenient.\<close>
 lemma bind_def':
   "(f >>= g) \<equiv>
-       \<lambda>s. ({(r'', s''). \<exists>(r', s') \<in> fst (f s). (r'', s'') \<in> fst (g r' s') },
-                     snd (f s) \<or> (\<exists>(r', s') \<in> fst (f s). snd (g r' s')))"
+       \<lambda>s. ({(r'', s''). \<exists>(r', s') \<in> fst (f s). (r'', s'') \<in> fst (g r' (with_env_of s s')) },
+                     snd (f s) \<or> (\<exists>(r', s') \<in> fst (f s). snd (g r' (with_env_of s s'))))"
   by (rule eq_reflection)
      (auto simp add: bind_def split_def Let_def)
+
+lemma with_env_of_mstate[simp]:
+  "with_env_of s (mstate s) = s"
+  by (cases s, auto)
 
 text \<open>Each monad satisfies at least the following three laws.\<close>
 
@@ -219,9 +276,9 @@ lemma bind_return[simp]:
 
 text \<open>@{term bind} is associative\<close>
 lemma bind_assoc:
-  fixes m :: "('a,'b) nondet_monad"
-  fixes f :: "'b \<Rightarrow> ('a,'c) nondet_monad"
-  fixes g :: "'c \<Rightarrow> ('a,'d) nondet_monad"
+  fixes m :: "('c, 's, 'a) nondet_monad"
+  fixes f :: "'a \<Rightarrow> ('c, 's, 'b) nondet_monad"
+  fixes g :: "'b \<Rightarrow> ('c, 's, 'd) nondet_monad"
   shows "(m >>= f) >>= g  =  m >>= (\<lambda>x. f x >>= g)"
   unfolding bind_def Let_def split_def
   by (auto intro: rev_image_eqI)
@@ -230,12 +287,12 @@ lemma bind_assoc:
 section \<open>Adding Exceptions\<close>
 
 text \<open>
-  The type @{typ "('s,'a) nondet_monad"} gives us nondeterminism and
+  The type @{typ "('c,'s,'a) nondet_monad"} gives us nondeterminism and
   failure. We now extend this monad with exceptional return values
   that abort normal execution, but can be handled explicitly.
   We use the sum type to indicate exceptions.
 
-  In @{typ "('s, 'e + 'a) nondet_monad"}, @{typ "'s"} is the state,
+  In @{typ "('c, 's, 'e + 'a) nondet_monad"}, @{typ "'s"} is the state,
   @{typ 'e} is an exception, and @{typ 'a} is a normal return value.
 
   This new type itself forms a monad again. Since type classes in
@@ -244,16 +301,16 @@ text \<open>
   in this monad. We call them @{text returnOk} (for normal return values)
   and @{text bindE} (for composition). We also define @{text throwError}
   to return an exceptional value.\<close>
-definition returnOk :: "'a \<Rightarrow> ('s, 'e + 'a) nondet_monad" where
+definition returnOk :: "'a \<Rightarrow> ('c, 's, 'e + 'a) nondet_monad" where
   "returnOk \<equiv> return o Inr"
 
-definition throwError :: "'e \<Rightarrow> ('s, 'e + 'a) nondet_monad" where
+definition throwError :: "'e \<Rightarrow> ('c, 's, 'e + 'a) nondet_monad" where
   "throwError \<equiv> return o Inl"
 
 text \<open>
   Lifting a function over the exception type: if the input is an
   exception, return that exception; otherwise continue execution.\<close>
-definition lift :: "('a \<Rightarrow> ('s, 'e + 'b) nondet_monad) \<Rightarrow> 'e +'a \<Rightarrow> ('s, 'e + 'b) nondet_monad" where
+definition lift :: "('a \<Rightarrow> ('c, 's, 'e + 'b) nondet_monad) \<Rightarrow> 'e +'a \<Rightarrow> ('c, 's, 'e + 'b) nondet_monad" where
   "lift f v \<equiv> case v of Inl e \<Rightarrow> throwError e | Inr v' \<Rightarrow> f v'"
 
 text \<open>
@@ -262,7 +319,7 @@ text \<open>
   the right-hand side is skipped if the left-hand side
   produced an exception.\<close>
 definition bindE ::
-  "('s, 'e + 'a) nondet_monad \<Rightarrow> ('a \<Rightarrow> ('s, 'e + 'b) nondet_monad) \<Rightarrow> ('s, 'e + 'b) nondet_monad"
+  "('c, 's, 'e + 'a) nondet_monad \<Rightarrow> ('a \<Rightarrow> ('c, 's, 'e + 'b) nondet_monad) \<Rightarrow> ('c, 's, 'e + 'b) nondet_monad"
   (infixl ">>=E" 60) where
   "f >>=E g \<equiv> f >>= lift g"
 
@@ -270,29 +327,29 @@ text \<open>
   Lifting a normal nondeterministic monad into the
   exception monad is achieved by always returning its
   result as normal result and never throwing an exception.\<close>
-definition liftE :: "('s,'a) nondet_monad \<Rightarrow> ('s, 'e+'a) nondet_monad" where
+definition liftE :: "('c,'s,'a) nondet_monad \<Rightarrow> ('c, 's, 'e+'a) nondet_monad" where
   "liftE f \<equiv> f >>= (\<lambda>r. return (Inr r))"
 
 text \<open>
   Since the underlying type and @{text return} function changed,
   we need new definitions for when and unless:\<close>
-definition whenE :: "bool \<Rightarrow> ('s, 'e + unit) nondet_monad \<Rightarrow> ('s, 'e + unit) nondet_monad" where
+definition whenE :: "bool \<Rightarrow> ('c, 's, 'e + unit) nondet_monad \<Rightarrow> ('c, 's, 'e + unit) nondet_monad" where
   "whenE P f \<equiv> if P then f else returnOk ()"
 
-definition unlessE :: "bool \<Rightarrow> ('s, 'e + unit) nondet_monad \<Rightarrow> ('s, 'e + unit) nondet_monad" where
+definition unlessE :: "bool \<Rightarrow> ('c, 's, 'e + unit) nondet_monad \<Rightarrow> ('c, 's, 'e + unit) nondet_monad" where
   "unlessE P f \<equiv> if P then returnOk () else f"
 
 text \<open>
   Throwing an exception when the parameter is @{term None}, otherwise
   returning @{term "v"} for @{term "Some v"}.\<close>
-definition throw_opt :: "'e \<Rightarrow> 'a option \<Rightarrow> ('s, 'e + 'a) nondet_monad" where
+definition throw_opt :: "'e \<Rightarrow> 'a option \<Rightarrow> ('c, 's, 'e + 'a) nondet_monad" where
   "throw_opt ex x \<equiv> case x of None \<Rightarrow> throwError ex | Some v \<Rightarrow> returnOk v"
 
 text \<open>
   Failure in the exception monad is redefined in the same way
   as @{const whenE} and @{const unlessE}, with @{term returnOk}
   instead of @{term return}.\<close>
-definition assertE :: "bool \<Rightarrow> ('a, 'e + unit) nondet_monad" where
+definition assertE :: "bool \<Rightarrow> ('c, 's, 'e + unit) nondet_monad" where
   "assertE P \<equiv> if P then returnOk () else fail"
 
 
@@ -417,25 +474,25 @@ lemma "doE x \<leftarrow> returnOk 1;
 section "Library of additional Monadic Functions and Combinators"
 
 text \<open>Lifting a normal function into the monad type:\<close>
-definition liftM :: "('a \<Rightarrow> 'b) \<Rightarrow> ('s,'a) nondet_monad \<Rightarrow> ('s, 'b) nondet_monad" where
+definition liftM :: "('a \<Rightarrow> 'b) \<Rightarrow> ('c, 's, 'a) nondet_monad \<Rightarrow> ('c, 's, 'b) nondet_monad" where
   "liftM f m \<equiv> do x \<leftarrow> m; return (f x) od"
 
 text \<open>The same for the exception monad:\<close>
-definition liftME :: "('a \<Rightarrow> 'b) \<Rightarrow> ('s,'e+'a) nondet_monad \<Rightarrow> ('s,'e+'b) nondet_monad" where
+definition liftME :: "('a \<Rightarrow> 'b) \<Rightarrow> ('c, 's, 'e+'a) nondet_monad \<Rightarrow> ('c, 's, 'e+'b) nondet_monad" where
   "liftME f m \<equiv> doE x \<leftarrow> m; returnOk (f x) odE"
 
 text \<open>Execute @{term f} for @{term "Some x"}, otherwise do nothing.\<close>
-definition maybeM :: "('a \<Rightarrow> ('s, unit) nondet_monad) \<Rightarrow> 'a option \<Rightarrow> ('s, unit) nondet_monad" where
+definition maybeM :: "('a \<Rightarrow> ('c, 's, unit) nondet_monad) \<Rightarrow> 'a option \<Rightarrow> ('c, 's, unit) nondet_monad" where
   "maybeM f y \<equiv> case y of Some x \<Rightarrow> f x | None \<Rightarrow> return ()"
 
 text \<open>Run a sequence of monads from left to right, ignoring return values.\<close>
-definition sequence_x :: "('s, 'a) nondet_monad list \<Rightarrow> ('s, unit) nondet_monad" where
+definition sequence_x :: "('c, 's, 'a) nondet_monad list \<Rightarrow> ('c, 's, unit) nondet_monad" where
   "sequence_x xs \<equiv> foldr (\<lambda>x y. x >>= (\<lambda>_. y)) xs (return ())"
 
 text \<open>
   Map a monadic function over a list by applying it to each element
   of the list from left to right, ignoring return values.\<close>
-definition mapM_x :: "('a \<Rightarrow> ('s,'b) nondet_monad) \<Rightarrow> 'a list \<Rightarrow> ('s, unit) nondet_monad" where
+definition mapM_x :: "('a \<Rightarrow> ('c, 's, 'b) nondet_monad) \<Rightarrow> 'a list \<Rightarrow> ('c, 's, unit) nondet_monad" where
   "mapM_x f xs \<equiv> sequence_x (map f xs)"
 
 text \<open>
@@ -443,55 +500,55 @@ text \<open>
   going through both lists simultaneously, left to right, ignoring
   return values.\<close>
 definition zipWithM_x ::
-  "('a \<Rightarrow> 'b \<Rightarrow> ('s,'c) nondet_monad) \<Rightarrow> 'a list \<Rightarrow> 'b list \<Rightarrow> ('s, unit) nondet_monad"
+  "('a \<Rightarrow> 'b \<Rightarrow> ('r,'s,'c) nondet_monad) \<Rightarrow> 'a list \<Rightarrow> 'b list \<Rightarrow> ('r, 's, unit) nondet_monad"
   where
   "zipWithM_x f xs ys \<equiv> sequence_x (zipWith f xs ys)"
 
 text \<open>
   The same three functions as above, but returning a list of
   return values instead of @{text unit}\<close>
-definition sequence :: "('s, 'a) nondet_monad list \<Rightarrow> ('s, 'a list) nondet_monad" where
+definition sequence :: "('c, 's, 'a) nondet_monad list \<Rightarrow> ('c, 's, 'a list) nondet_monad" where
   "sequence xs \<equiv> let mcons = (\<lambda>p q. p >>= (\<lambda>x. q >>= (\<lambda>y. return (x#y))))
                  in foldr mcons xs (return [])"
 
-definition mapM :: "('a \<Rightarrow> ('s,'b) nondet_monad) \<Rightarrow> 'a list \<Rightarrow> ('s, 'b list) nondet_monad" where
+definition mapM :: "('a \<Rightarrow> ('c, 's,'b) nondet_monad) \<Rightarrow> 'a list \<Rightarrow> ('c, 's, 'b list) nondet_monad" where
   "mapM f xs \<equiv> sequence (map f xs)"
 
 definition zipWithM ::
-  "('a \<Rightarrow> 'b \<Rightarrow> ('s,'c) nondet_monad) \<Rightarrow> 'a list \<Rightarrow> 'b list \<Rightarrow> ('s, 'c list) nondet_monad"
+  "('a \<Rightarrow> 'b \<Rightarrow> ('r,'s,'c) nondet_monad) \<Rightarrow> 'a list \<Rightarrow> 'b list \<Rightarrow> ('r, 's, 'c list) nondet_monad"
   where
   "zipWithM f xs ys \<equiv> sequence (zipWith f xs ys)"
 
 definition foldM ::
-  "('b \<Rightarrow> 'a \<Rightarrow> ('s, 'a) nondet_monad) \<Rightarrow> 'b list \<Rightarrow> 'a \<Rightarrow> ('s, 'a) nondet_monad"
+  "('b \<Rightarrow> 'a \<Rightarrow> ('r, 's, 'a) nondet_monad) \<Rightarrow> 'b list \<Rightarrow> 'a \<Rightarrow> ('r, 's, 'a) nondet_monad"
   where
   "foldM m xs a \<equiv> foldr (\<lambda>p q. q >>= m p) xs (return a) "
 
 definition foldME ::
-  "('b \<Rightarrow> 'a \<Rightarrow> ('s,('e + 'b)) nondet_monad) \<Rightarrow> 'b \<Rightarrow> 'a list \<Rightarrow> ('s, ('e + 'b)) nondet_monad"
+  "('b \<Rightarrow> 'a \<Rightarrow> ('c, 's, ('e + 'b)) nondet_monad) \<Rightarrow> 'b \<Rightarrow> 'a list \<Rightarrow> ('c, 's, ('e + 'b)) nondet_monad"
   where
   "foldME m a xs \<equiv> foldr (\<lambda>p q. q >>=E swp m p) xs (returnOk a)"
 
 text \<open>
   The sequence and map functions above for the exception monad, with and without
   lists of return value\<close>
-definition sequenceE_x :: "('s, 'e+'a) nondet_monad list \<Rightarrow> ('s, 'e+unit) nondet_monad" where
+definition sequenceE_x :: "('c, 's, 'e+'a) nondet_monad list \<Rightarrow> ('c, 's, 'e+unit) nondet_monad" where
   "sequenceE_x xs \<equiv> foldr (\<lambda>x y. doE _ <- x; y odE) xs (returnOk ())"
 
-definition mapME_x :: "('a \<Rightarrow> ('s,'e+'b) nondet_monad) \<Rightarrow> 'a list \<Rightarrow> ('s,'e+unit) nondet_monad" where
+definition mapME_x :: "('a \<Rightarrow> ('c, 's,'e+'b) nondet_monad) \<Rightarrow> 'a list \<Rightarrow> ('c, 's,'e+unit) nondet_monad" where
   "mapME_x f xs \<equiv> sequenceE_x (map f xs)"
 
-definition sequenceE :: "('s, 'e+'a) nondet_monad list \<Rightarrow> ('s, 'e+'a list) nondet_monad" where
+definition sequenceE :: "('c, 's, 'e+'a) nondet_monad list \<Rightarrow> ('c, 's, 'e+'a list) nondet_monad" where
   "sequenceE xs \<equiv> let mcons = (\<lambda>p q. p >>=E (\<lambda>x. q >>=E (\<lambda>y. returnOk (x#y))))
                    in foldr mcons xs (returnOk [])"
 
 definition mapME ::
-  "('a \<Rightarrow> ('s,'e+'b) nondet_monad) \<Rightarrow> 'a list \<Rightarrow> ('s,'e+'b list) nondet_monad"
+  "('a \<Rightarrow> ('c,'s,'e+'b) nondet_monad) \<Rightarrow> 'a list \<Rightarrow> ('c,'s,'e+'b list) nondet_monad"
   where
   "mapME f xs \<equiv> sequenceE (map f xs)"
 
 text \<open>Filtering a list using a monadic function as predicate:\<close>
-primrec filterM :: "('a \<Rightarrow> ('s, bool) nondet_monad) \<Rightarrow> 'a list \<Rightarrow> ('s, 'a list) nondet_monad" where
+primrec filterM :: "('a \<Rightarrow> ('c,'s, bool) nondet_monad) \<Rightarrow> 'a list \<Rightarrow> ('c, 's, 'a list) nondet_monad" where
   "filterM P []       = return []"
 | "filterM P (x # xs) = do
      b  <- P x;
@@ -521,7 +578,7 @@ text \<open>
   Turning an exception monad into a normal state monad
   by catching and handling any potential exceptions:\<close>
 definition catch ::
-  "('s, 'e + 'a) nondet_monad \<Rightarrow> ('e \<Rightarrow> ('s, 'a) nondet_monad) \<Rightarrow> ('s, 'a) nondet_monad"
+  "('c, 's, 'e + 'a) nondet_monad \<Rightarrow> ('e \<Rightarrow> ('c, 's, 'a) nondet_monad) \<Rightarrow> ('c, 's, 'a) nondet_monad"
   (infix "<catch>" 10) where
   "f <catch> handler \<equiv>
      do x \<leftarrow> f;
@@ -535,7 +592,7 @@ text \<open>
   The handler may throw a type of exceptions different from
   the left side.\<close>
 definition handleE' ::
-  "('s, 'e1 + 'a) nondet_monad \<Rightarrow> ('e1 \<Rightarrow> ('s, 'e2 + 'a) nondet_monad) \<Rightarrow> ('s, 'e2 + 'a) nondet_monad"
+  "('c, 's, 'e1 + 'a) nondet_monad \<Rightarrow> ('e1 \<Rightarrow> ('c, 's, 'e2 + 'a) nondet_monad) \<Rightarrow> ('c, 's, 'e2 + 'a) nondet_monad"
   (infix "<handle2>" 10) where
   "f <handle2> handler \<equiv>
    do
@@ -547,10 +604,10 @@ definition handleE' ::
 
 text \<open>
   A type restriction of the above that is used more commonly in
-  practice: the exception handle (potentially) throws exception
+  practice: the exception handler (potentially) throws an exception
   of the same type as the left-hand side.\<close>
 definition handleE ::
-  "('s, 'x + 'a) nondet_monad \<Rightarrow> ('x \<Rightarrow> ('s, 'x + 'a) nondet_monad) \<Rightarrow> ('s, 'x + 'a) nondet_monad"
+  "('c, 's, 'x + 'a) nondet_monad \<Rightarrow> ('x \<Rightarrow> ('c, 's, 'x + 'a) nondet_monad) \<Rightarrow> ('c, 's, 'x + 'a) nondet_monad"
   (infix "<handle>" 10) where
   "handleE \<equiv> handleE'"
 
@@ -558,8 +615,8 @@ text \<open>
   Handling exceptions, and additionally providing a continuation
   if the left-hand side throws no exception:\<close>
 definition handle_elseE ::
-  "('s, 'e + 'a) nondet_monad \<Rightarrow> ('e \<Rightarrow> ('s, 'ee + 'b) nondet_monad) \<Rightarrow>
-   ('a \<Rightarrow> ('s, 'ee + 'b) nondet_monad) \<Rightarrow> ('s, 'ee + 'b) nondet_monad" ("_ <handle> _ <else> _" 10)
+  "('c, 's, 'e + 'a) nondet_monad \<Rightarrow> ('e \<Rightarrow> ('c, 's, 'ee + 'b) nondet_monad) \<Rightarrow>
+   ('a \<Rightarrow> ('c, 's, 'ee + 'b) nondet_monad) \<Rightarrow> ('c, 's, 'ee + 'b) nondet_monad" ("_ <handle> _ <else> _" 10)
   where
   "f <handle> handler <else> continue \<equiv>
    do v \<leftarrow> f;
@@ -573,43 +630,48 @@ text \<open>
   Loops are handled using the following inductive predicate;
   non-termination is represented using the failure flag of the
   monad.\<close>
-
 inductive_set whileLoop_results ::
-  "('r \<Rightarrow> 's \<Rightarrow> bool) \<Rightarrow> ('r \<Rightarrow> ('s, 'r) nondet_monad) \<Rightarrow> ((('r \<times> 's) option) \<times> (('r \<times> 's) option)) set"
-  for C B where
-    "\<lbrakk> \<not> C r s \<rbrakk> \<Longrightarrow> (Some (r, s), Some (r, s)) \<in> whileLoop_results C B"
-  | "\<lbrakk> C r s; snd (B r s) \<rbrakk> \<Longrightarrow> (Some (r, s), None) \<in> whileLoop_results C B"
-  | "\<lbrakk> C r s; (r', s') \<in> fst (B r s); (Some (r', s'), z) \<in> whileLoop_results C B  \<rbrakk>
-       \<Longrightarrow> (Some (r, s), z) \<in> whileLoop_results C B"
+  "('r \<Rightarrow> ('c,'s) mpred) \<Rightarrow> ('r \<Rightarrow> ('c, 's, 'r) nondet_monad) \<Rightarrow> 'c \<Rightarrow>
+   ((('r \<times> 's) option) \<times> (('r \<times> 's) option)) set"
+  for C B c where
+    "\<lbrakk> \<not> C r (monad_state c s) \<rbrakk> \<Longrightarrow> (Some (r, s), Some (r, s)) \<in> whileLoop_results C B c"
+  | "\<lbrakk> C  r (monad_state c s); snd (B r (monad_state c s)) \<rbrakk>
+     \<Longrightarrow> (Some (r, s), None) \<in> whileLoop_results C B c"
+  | "\<lbrakk> C r (monad_state c s); (r', s') \<in> fst (B r (monad_state c s));
+       (Some (r', s'), z) \<in> whileLoop_results C B c \<rbrakk>
+     \<Longrightarrow> (Some (r, s), z) \<in> whileLoop_results C B c"
 
-inductive_cases whileLoop_results_cases_valid: "(Some x, Some y) \<in> whileLoop_results C B"
-inductive_cases whileLoop_results_cases_fail: "(Some x, None) \<in> whileLoop_results C B"
-inductive_simps whileLoop_results_simps: "(Some x, y) \<in> whileLoop_results C B"
-inductive_simps whileLoop_results_simps_valid: "(Some x, Some y) \<in> whileLoop_results C B"
-inductive_simps whileLoop_results_simps_start_fail[simp]: "(None, x) \<in> whileLoop_results C B"
+inductive_cases whileLoop_results_cases_valid: "(Some x, Some y) \<in> whileLoop_results C B c"
+inductive_cases whileLoop_results_cases_fail: "(Some x, None) \<in> whileLoop_results C B c"
+inductive_simps whileLoop_results_simps: "(Some x, y) \<in> whileLoop_results C B c"
+inductive_simps whileLoop_results_simps_valid: "(Some x, Some y) \<in> whileLoop_results C B c"
+inductive_simps whileLoop_results_simps_start_fail[simp]: "(None, x) \<in> whileLoop_results C B c"
 
 inductive whileLoop_terminates ::
-  "('r \<Rightarrow> 's \<Rightarrow> bool) \<Rightarrow> ('r \<Rightarrow> ('s, 'r) nondet_monad) \<Rightarrow> 'r \<Rightarrow> 's \<Rightarrow> bool"
-  for C B where
-    "\<not> C r s \<Longrightarrow> whileLoop_terminates C B r s"
-  | "\<lbrakk> C r s; \<forall>(r', s') \<in> fst (B r s). whileLoop_terminates C B r' s' \<rbrakk>
-        \<Longrightarrow> whileLoop_terminates C B r s"
+  "('r \<Rightarrow> ('c,'s) mpred) \<Rightarrow> ('r \<Rightarrow> ('c, 's, 'r) nondet_monad) \<Rightarrow> 'c \<Rightarrow> 'r \<Rightarrow> 's \<Rightarrow> bool"
+  for C B c where
+    "\<not> C r (monad_state c s) \<Longrightarrow> whileLoop_terminates C B c r s"
+  | "\<lbrakk> C r (monad_state c s);
+       \<forall>(r', s') \<in> fst (B r (monad_state c s)). whileLoop_terminates C B c r' s' \<rbrakk>
+     \<Longrightarrow> whileLoop_terminates C B c r s"
 
-inductive_cases whileLoop_terminates_cases: "whileLoop_terminates C B r s"
-inductive_simps whileLoop_terminates_simps: "whileLoop_terminates C B r s"
+inductive_cases whileLoop_terminates_cases: "whileLoop_terminates C B c r s"
+inductive_simps whileLoop_terminates_simps: "whileLoop_terminates C B c r s"
 
 definition whileLoop ::
-  "('a \<Rightarrow> 'b \<Rightarrow> bool) \<Rightarrow> ('a \<Rightarrow> ('b, 'a) nondet_monad) \<Rightarrow> 'a \<Rightarrow> ('b, 'a) nondet_monad"
+  "('a \<Rightarrow> ('c,'s) mpred) \<Rightarrow> ('a \<Rightarrow> ('c, 's, 'a) nondet_monad) \<Rightarrow> 'a \<Rightarrow> ('c, 's, 'a) nondet_monad"
   where
   "whileLoop C B \<equiv> \<lambda>r s.
-     ({(r',s'). (Some (r, s), Some (r', s')) \<in> whileLoop_results C B},
-      (Some (r, s), None) \<in> whileLoop_results C B \<or> \<not>whileLoop_terminates C B r s)"
+     ({(r',s'). (Some (r, mstate s), Some (r', s')) \<in> whileLoop_results C B (env s)},
+      (Some (r, mstate s), None) \<in> whileLoop_results C B (env s) \<or>
+      \<not>whileLoop_terminates C B (env s) r (mstate s))"
 
 notation (output)
   whileLoop  ("(whileLoop (_)//  (_))" [1000, 1000] 1000)
 
 definition whileLoopE ::
-  "('r \<Rightarrow> 's \<Rightarrow> bool) \<Rightarrow> ('r \<Rightarrow> ('s, 'e + 'r) nondet_monad) \<Rightarrow> 'r \<Rightarrow> 's \<Rightarrow> (('e + 'r) \<times> 's) set \<times> bool"
+  "('r \<Rightarrow> ('c,'s) mpred) \<Rightarrow> ('r \<Rightarrow> ('c, 's, 'e + 'r) nondet_monad) \<Rightarrow>
+   'r \<Rightarrow> ('c, 's, 'e + 'r) nondet_monad"
   where
   "whileLoopE C body \<equiv>
      \<lambda>r. whileLoop (\<lambda>r s. (case r of Inr v \<Rightarrow> C v s | _ \<Rightarrow> False)) (lift body) (Inr r)"
@@ -620,11 +682,11 @@ notation (output)
 
 section "Combinators that have conditions with side effects"
 
-definition notM :: "('s, bool) nondet_monad \<Rightarrow> ('s, bool) nondet_monad" where
+definition notM :: "('c, 's, bool) nondet_monad \<Rightarrow> ('c, 's, bool) nondet_monad" where
   "notM m = do c \<leftarrow> m; return (\<not> c) od"
 
 definition whileM ::
-  "('s, bool) nondet_monad \<Rightarrow> ('s, 'a) nondet_monad \<Rightarrow> ('s, unit) nondet_monad"
+  "('c, 's, bool) nondet_monad \<Rightarrow> ('c, 's, 'a) nondet_monad \<Rightarrow> ('c, 's, unit) nondet_monad"
   where
   "whileM C B \<equiv> do
     c \<leftarrow> C;
@@ -633,7 +695,7 @@ definition whileM ::
   od"
 
 definition ifM ::
-  "('s, bool) nondet_monad \<Rightarrow> ('s, 'a) nondet_monad \<Rightarrow> ('s, 'a) nondet_monad \<Rightarrow> ('s, 'a) nondet_monad"
+  "('c, 's, bool) nondet_monad \<Rightarrow> ('c, 's, 'a) nondet_monad \<Rightarrow> ('c, 's, 'a) nondet_monad \<Rightarrow> ('c, 's, 'a) nondet_monad"
   where
   "ifM test t f = do
     c \<leftarrow> test;
@@ -641,8 +703,8 @@ definition ifM ::
    od"
 
 definition ifME ::
-  "('a, 'b + bool) nondet_monad \<Rightarrow> ('a, 'b + 'c) nondet_monad \<Rightarrow> ('a, 'b + 'c) nondet_monad
-   \<Rightarrow> ('a, 'b + 'c) nondet_monad"
+  "('c, 's, 'a + bool) nondet_monad \<Rightarrow> ('c, 's, 'a + 'b) nondet_monad \<Rightarrow> ('c, 's, 'a + 'b) nondet_monad
+   \<Rightarrow> ('c, 's, 'a + 'b) nondet_monad"
   where
   "ifME test t f = doE
     c \<leftarrow> test;
@@ -650,17 +712,17 @@ definition ifME ::
    odE"
 
 definition whenM ::
-  "('s, bool) nondet_monad \<Rightarrow> ('s, unit) nondet_monad \<Rightarrow> ('s, unit) nondet_monad"
+  "('c, 's, bool) nondet_monad \<Rightarrow> ('c, 's, unit) nondet_monad \<Rightarrow> ('c, 's, unit) nondet_monad"
   where
   "whenM t m = ifM t m (return ())"
 
 definition orM ::
-  "('s, bool) nondet_monad \<Rightarrow> ('s, bool) nondet_monad \<Rightarrow> ('s, bool) nondet_monad"
+  "('c, 's, bool) nondet_monad \<Rightarrow> ('c, 's, bool) nondet_monad \<Rightarrow> ('c, 's, bool) nondet_monad"
   where
   "orM a b = ifM a (return True) b"
 
 definition andM ::
-  "('s, bool) nondet_monad \<Rightarrow> ('s, bool) nondet_monad \<Rightarrow> ('s, bool) nondet_monad"
+  "('c, 's, bool) nondet_monad \<Rightarrow> ('c, 's, bool) nondet_monad \<Rightarrow> ('c, 's, bool) nondet_monad"
   where
   "andM a b = ifM a b (return False)"
 
