lib/Monads/nondet/Nondet_While_Loop_Rules_Completeness.thy
@@ -15,22 +15,23 @@ theory Nondet_While_Loop_Rules_Completeness
 begin
 
 lemma whileLoop_rule_strong_complete:
-  "(\<lbrace> \<lambda>s'. s' = s \<rbrace> whileLoop C B r \<lbrace> \<lambda>r s. (r, s) \<in> fst Q \<rbrace>
-        \<and> (\<forall>r'' s''. (r'', s'') \<in> fst Q \<longrightarrow> \<lbrace> \<lambda>s'. s' = s \<rbrace> whileLoop C B r \<exists>\<lbrace> \<lambda>r s. r = r'' \<and> s = s'' \<rbrace>)
-        \<and> (snd Q \<longrightarrow> snd (whileLoop C B r s))
-        \<and> (\<not> snd Q \<longrightarrow> \<lbrace> \<lambda>s'. s' = s \<rbrace> whileLoop C B r \<lbrace> \<lambda>_ _. True \<rbrace>!))
-    = (whileLoop C B r s = Q)"
+  "(\<lbrace>\<lambda>s'. s' = s\<rbrace> whileLoop C B r \<lbrace>\<lambda>r s. (r, mstate s) \<in> fst Q\<rbrace> \<and>
+    (\<forall>r'' s''. (r'', mstate s'') \<in> fst Q \<and> env s'' = env s \<longrightarrow>
+               \<lbrace>\<lambda>s'. s' = s\<rbrace> whileLoop C B r \<exists>\<lbrace>\<lambda>r s. r = r'' \<and> s = s''\<rbrace>) \<and>
+    (snd Q \<longrightarrow> snd (whileLoop C B r s)) \<and>
+    (\<not> snd Q \<longrightarrow> \<lbrace>\<lambda>s'. s' = s\<rbrace> whileLoop C B r \<lbrace>\<lambda>_ _. True\<rbrace>!)) =
+   (whileLoop C B r s = Q)"
   apply (rule iffI)
-   apply (rule whileLoop_rule_strong, auto)[1]
-  apply (clarsimp simp: valid_def exs_valid_def validNF_alt_def)
-  apply force
+   apply (rule whileLoop_rule_strong; clarsimp)
+   apply (clarsimp simp: exs_valid_def)
+   apply (smt (verit) case_prod_beta select_convs)
+  apply (force simp: valid_def exs_valid_def validNF_alt_def)
   done
 
 lemma valid_whileLoop_complete:
-  "(\<exists>I.
-       (\<forall>s. P r s \<longrightarrow> I r s )
-     \<and> (\<forall>r. \<lbrace> \<lambda>s. I r s \<and> C r s \<rbrace> B r \<lbrace> I \<rbrace>)
-     \<and> (\<forall>r s. ( I r s \<and> \<not> C r s ) \<longrightarrow> Q r s))
+  "(\<exists>I. (\<forall>s. P r s \<longrightarrow> I r s )
+        \<and> (\<forall>r. \<lbrace> \<lambda>s. I r s \<and> C r s \<rbrace> B r \<lbrace> I \<rbrace>)
+        \<and> (\<forall>r s. ( I r s \<and> \<not> C r s ) \<longrightarrow> Q r s))
     = \<lbrace> P r \<rbrace> whileLoop C B r \<lbrace> Q \<rbrace>"
   apply (rule iffI)
    apply clarsimp
@@ -43,7 +44,7 @@ lemma valid_whileLoop_complete:
    apply clarsimp
    apply (rename_tac a b)
    apply (subst (asm) (2) whileLoop_unroll)
-   apply (case_tac "C a b")
+   apply (case_tac "C a (with_env_of s b)")
     apply (clarsimp simp: valid_def bind_def' Bex_def condition_def split: if_split_asm)
     apply force
    apply (clarsimp simp: valid_def bind_def' Bex_def condition_def split: if_split_asm)
@@ -56,7 +57,7 @@ lemma validNF_whileLoop_complete:
   "(\<exists>I R.
        (\<forall>s. P r s \<longrightarrow> I r s )
      \<and> (\<forall>r s. \<lbrace>\<lambda>s'. I r s' \<and> C r s' \<and> s' = s\<rbrace> B r \<lbrace>\<lambda>r' s'. I r' s' \<and> ((r', s'), r, s) \<in> R\<rbrace>!)
-     \<and> (wf R)
+     \<and> wf R
      \<and> (\<forall>r s. ( I r s \<and> \<not> C r s ) \<longrightarrow> Q r s))
     = \<lbrace> P r \<rbrace> whileLoop C B r \<lbrace> Q \<rbrace>!"
   (is "(\<exists>I R. ?LHS I R) = ?RHS")
@@ -68,20 +69,21 @@ proof (rule iffI)
     by auto
 
   thus ?RHS
-    by - (rule validNF_whileLoop[where I=I and R=R], auto)
+    by - (rule validNF_whileLoop[where I=I], auto)
 next
   assume loop: "?RHS"
 
   define I where "I \<equiv> \<lambda>r s. \<lbrace> \<lambda>s'. s' = s \<rbrace> whileLoop C B r \<lbrace> \<lambda>r s. Q r s \<rbrace>!"
-  define R where "R \<equiv> {(x, y). C (fst y) (snd y) \<and> x \<in> fst (B (fst y) (snd y)) \<and>
-                                whileLoop_terminates C B (fst y) (snd y)}"
+  define R where "R \<equiv> {(x, y). C (fst y) (snd y) \<and> (fst x, mstate (snd x)) \<in> fst (B (fst y) (snd y)) \<and>
+                               env (snd x) = env (snd y) \<and>
+                               whileLoop_terminates C B (env (snd y)) (fst y) (mstate (snd y))}"
 
-  have "wf R"
+  have wf: "wf R"
     using R_def whileLoop_terminates_wf
     by auto
 
   have start: "\<And>s. P r s \<Longrightarrow> I r s"
-    by (metis (full_types) I_def loop validNF_weaken_pre)
+    using I_def loop validNF_chain by fastforce
 
   have fin: "\<And>r s. \<lbrakk> I r s; \<not> C r s \<rbrakk> \<Longrightarrow> Q r s"
     apply (unfold I_def)
@@ -95,7 +97,7 @@ next
              (is "\<And>r s. \<lbrace> ?pre r s \<rbrace> B r \<lbrace> ?post r s \<rbrace>!")
   proof -
     have inv_step:
-        "\<And>r s r' s'. \<lbrakk> I r s; C r s; (r', s') \<in> fst (B r s) \<rbrakk> \<Longrightarrow> I r' s'"
+        "\<And>r s r' s'. \<lbrakk> I r s; C r s; (r', s') \<in> fst (B r s) \<rbrakk> \<Longrightarrow> I r' (with_env_of s s')"
       apply (clarsimp simp: I_def)
       apply (subst (asm) whileLoop_unroll)
       apply (clarsimp simp: condition_def bind_def' validNF_alt_def)
@@ -103,7 +105,7 @@ next
       done
 
     have R_step:
-        "\<And>r s r' s'. \<lbrakk> I r s; C r s; (r', s') \<in> fst (B r s) \<rbrakk> \<Longrightarrow> ((r', s'), (r, s)) \<in> R"
+        "\<And>r s r' s'. \<lbrakk> I r s; C r s; (r', s') \<in> fst (B r s) \<rbrakk> \<Longrightarrow> ((r', with_env_of s s'), (r, s)) \<in> R"
       apply (clarsimp simp: I_def R_def)
       apply (clarsimp simp: validNF_alt_def whileLoop_def)
       done
@@ -115,10 +117,10 @@ next
       apply (drule (1) snd_whileLoop_first_step)
       apply simp
       done
-    qed
+  qed
 
   show "\<exists>I' R'. ?LHS I' R'"
-    using \<open>wf R\<close> start fin step
+    using wf start fin step
     by blast
 qed
 
@@ -126,25 +128,24 @@ qed
 lemma snd_whileLoop_complete:
   shows "snd (whileLoop C B r s) =
               (\<exists>I. I r s \<and> C r s \<and>
-                   (\<forall>r. \<lbrace> \<lambda>s. I r s \<and> C r s \<and> \<not> snd (B r s) \<rbrace>
-                            B r \<exists>\<lbrace> \<lambda>r s. C r s \<and> I r s \<rbrace>))"
+                   (\<forall>r. \<lbrace> \<lambda>s. I r s \<and> C r s \<and> \<not> snd (B r s) \<rbrace> B r \<exists>\<lbrace> \<lambda>r s. C r s \<and> I r s \<rbrace>))"
   (is "?LHS = ?RHS")
 proof (rule iffI)
   assume "?LHS"
   thus "?RHS"
     apply (clarsimp simp: whileLoop_def)
     apply (erule disjE)
-     apply (rule exI [where x="\<lambda>r s. (Some (r, s), None) \<in> whileLoop_results C B"])
+     apply (rule exI [where x="\<lambda>r s. (Some (r, mstate s), None) \<in> whileLoop_results C B (env s)"])
      apply (intro conjI)
        apply simp
-      apply (metis Pair_inject whileLoop_results_cases_fail)
+      apply (force elim: whileLoop_results_cases_fail)
      apply (clarsimp simp: exs_valid_def)
      apply (erule whileLoop_results_cases_fail, fastforce)
      apply clarsimp
      apply (erule bexI [rotated])
      apply clarsimp
      apply (metis fst_conv snd_conv whileLoop_results_cases_fail)
-    apply (rule exI [where x="\<lambda>r s. \<not> whileLoop_terminates C B r s"])
+    apply (rule exI [where x="\<lambda>r s. \<not> whileLoop_terminates C B (env s) r (mstate s)"])
     apply clarsimp
     apply (rule conjI)
      apply (subst (asm)  whileLoop_terminates_simps)
@@ -167,51 +168,55 @@ next
 qed
 
 lemma not_snd_whileLoop_complete:
-  shows "(\<not> snd (whileLoop C B r s)) = (\<exists>I R . I r s \<and> wf R \<and>
-           (\<forall>r s r' s'. (I r s \<and> C r s \<and> (r', s') \<in> fst (B r s)) \<longrightarrow> I r' s')
+  "(\<not> snd (whileLoop C B r s)) =
+   (\<exists>I R . I r s \<and> wf R
+           \<and> (\<forall>r s r' s'. (I r s \<and> C r s \<and> (r', s') \<in> fst (B r s)) \<longrightarrow> I r' (with_env_of s s'))
            \<and> (\<forall>r s. I r s \<and> C r s \<longrightarrow> \<not> snd (B r s))
-           \<and> (\<forall>r s r' s'. I r s \<and> C r s \<and> (r', s') \<in> fst (B r s) \<longrightarrow> ((r', s'), (r, s)) \<in> R))"
+           \<and> (\<forall>r s r' s'. I r s \<and> C r s \<and> (r', s') \<in> fst (B r s) \<longrightarrow>
+                          ((r', with_env_of s s'), (r, s)) \<in> R))"
    (is "?LHS = ?RHS")
 proof (rule iffI)
   assume "?RHS"
   thus "?LHS"
-    apply (clarsimp)
-    apply (erule make_pos_goal, rule not_snd_whileLoop)
-      apply assumption
-     defer
-     apply assumption
+    apply clarsimp
+    apply (erule make_pos_goal, rule not_snd_whileLoop; assumption?)
     apply (clarsimp simp: validNF_def no_fail_def valid_def)
     done
 next
   assume no_fail: "?LHS"
   define I where "I \<equiv> \<lambda>r s. \<not> snd (whileLoop C B r s)"
-  define R where "R \<equiv> {((r', s'), (r, s)). C r s \<and> (r', s') \<in> fst (B r s) \<and>
-                                            whileLoop_terminates C B r s}"
+  define R where "R \<equiv> {((r', s'), (r, s)). C r s \<and> (r', mstate s') \<in> fst (B r s) \<and>
+                                            env s' = env s \<and>
+                                            whileLoop_terminates C B (env s) r (mstate s)}"
 
   have "I r s"
     by (clarsimp simp: I_def no_fail)
 
-  moreover have "wf R"
+  moreover
+  have "wf R"
     apply (rule wf_subset [OF whileLoop_terminates_wf [where C=C and B=B]])
     apply (clarsimp simp: R_def)
     done
 
-  moreover have "\<And>r s r' s'. \<lbrakk> I r s; C r s; (r', s') \<in> fst (B r s) \<rbrakk> \<Longrightarrow> I r' s'"
+  moreover
+  have "\<And>r s r' s'. \<lbrakk> I r s; C r s; (r', s') \<in> fst (B r s) \<rbrakk> \<Longrightarrow> I r' (with_env_of s s')"
     apply (clarsimp simp: I_def whileLoop_def)
     apply (rule conjI)
-     apply (metis whileLoop_results_simps)
+     apply (metis whileLoop_results.intros(3) with_env_of_mstate)
     apply (erule whileLoop_terminates_cases)
      apply clarsimp
     apply fastforce
     done
 
-  moreover have "\<And>r s. \<lbrakk> I r s; C r s \<rbrakk> \<Longrightarrow> \<not> snd (B r s)"
+  moreover
+  have "\<And>r s. \<lbrakk> I r s; C r s \<rbrakk> \<Longrightarrow> \<not> snd (B r s)"
     apply (clarsimp simp: I_def)
     apply (subst (asm) whileLoop_unroll)
     apply (clarsimp simp: condition_true bind_def)
     done
 
-  moreover have "\<And>r s r' s'. \<lbrakk> I r s; C r s; (r', s') \<in> fst (B r s) \<rbrakk> \<Longrightarrow> ((r', s'), (r, s)) \<in> R"
+  moreover
+  have "\<And>r s r' s'. \<lbrakk> I r s; C r s; (r', s') \<in> fst (B r s) \<rbrakk> \<Longrightarrow> ((r', with_env_of s s'), (r, s)) \<in> R"
     apply (clarsimp simp: R_def)
     apply (metis I_def snd_conv whileLoop_def)
     done
@@ -221,17 +226,18 @@ next
 qed
 
 
-fun valid_path
-where
+fun valid_path where
     "valid_path C B [] = False"
-  | "valid_path C B [x] = (\<not> C (fst x) (snd x))"
-  | "valid_path C B (x#y#xs) = ((C (fst x) (snd x) \<and> y \<in> fst (B (fst x) (snd x)) \<and> valid_path C B (y#xs)))"
+  | "valid_path C B [x] = (\<not>C (fst x) (snd x))"
+  | "valid_path C B (x#y#xs) = ((C (fst x) (snd x) \<and> (fst y, mstate (snd y)) \<in> fst (B (fst x) (snd x)) \<and>
+                                env (snd y) = env (snd x) \<and> valid_path C B (y#xs)))"
 
 lemma valid_path_not_empty:
   "valid_path C B xs \<Longrightarrow> xs \<noteq> []"
   by clarsimp
 
-definition "shortest_path_length C B x Q \<equiv>
+definition shortest_path_length where
+  "shortest_path_length C B x Q \<equiv>
         (LEAST n. \<exists>l. valid_path C B l \<and> hd l = x \<and> Q (fst (last l)) (snd (last l)) \<and> length l = n)"
 
 lemma shortest_path_length_same [simp]:
@@ -246,13 +252,10 @@ lemma shortest_path_length_same [simp]:
 
 lemma valid_path_simp:
   "valid_path C B l =
-        (((\<exists>r s. l = [(r, s)] \<and> \<not> C r s) \<or>
-              (\<exists>r s r' s' xs. l = (r, s)#(r', s')#xs \<and> C r s \<and> (r', s') \<in> fst (B r s) \<and> valid_path C B ((r', s')#xs))))"
-  apply (cases l rule: remdups_adj.cases)
-    apply clarsimp
-   apply clarsimp
-  apply clarsimp
-  done
+     ((\<exists>r s. l = [(r, s)] \<and> \<not>C r s) \<or>
+             (\<exists>r s r' s' xs. l = (r, s)#(r', s')#xs \<and> C r s \<and> (r', mstate s') \<in> fst (B r s) \<and>
+                             env s' = env s \<and> valid_path C B ((r', s')#xs)))"
+  by (cases l rule: remdups_adj.cases; clarsimp)
 
 lemma path_exists:
   assumes path: "\<lbrace> \<lambda>s'. s' = s \<rbrace> whileLoop C B r \<exists>\<lbrace> Q \<rbrace>"
@@ -261,7 +264,7 @@ proof -
   {
     fix r' s'
     assume x: "(r', s') \<in> fst (whileLoop C B r s)"
-    assume y: "Q r' s'"
+    assume y: "Q r' (with_env_of s s')"
     have ?thesis
       using x y
     proof (induct rule: in_whileLoop_induct)
@@ -318,59 +321,48 @@ next
   case (Cons a l)
   then show ?case
     apply clarsimp
-    apply rule
+    apply (rule conjI)
      apply clarsimp
      apply (subst whileLoop_unroll)
      apply (clarsimp simp: condition_def bind_def' exs_valid_def return_def)
     apply clarsimp
     apply (subst whileLoop_unroll)
     apply (clarsimp simp: condition_def bind_def' exs_valid_def return_def)
-    apply rule
-     apply (clarsimp split: prod.splits)
-     apply (cases l)
-      apply clarsimp
-     apply (clarsimp split del: if_split)
-     apply (erule bexI[rotated])
-     apply clarsimp
-    apply clarsimp
-    apply (cases l; clarsimp)
+    apply (cases l; clarsimp split del: if_split split: prod.splits)
+    apply (metis fst_conv snd_conv with_env_of_mstate)
     done
 qed
 
 lemma shortest_path_gets_shorter:
-  "\<lbrakk> \<lbrace> \<lambda>s'. s' = s \<rbrace> whileLoop C B r \<exists>\<lbrace> Q \<rbrace>;
-       C r s \<rbrakk>
-     \<Longrightarrow> \<exists>(r', s') \<in> fst (B r s).
-                shortest_path_length C B (r', s') Q < shortest_path_length C B (r, s) Q
-                 \<and> \<lbrace> \<lambda>s. s = s' \<rbrace> whileLoop C B r' \<exists>\<lbrace> Q \<rbrace>"
+  "\<lbrakk> \<lbrace> \<lambda>s'. s' = s \<rbrace> whileLoop C B r \<exists>\<lbrace> Q \<rbrace>; C r s \<rbrakk> \<Longrightarrow>
+   \<exists>(r', s') \<in> fst (B r s).
+     shortest_path_length C B (r', with_env_of s s') Q < shortest_path_length C B (r, s) Q
+     \<and> \<lbrace> \<lambda>s''. s'' = with_env_of s s' \<rbrace> whileLoop C B r' \<exists>\<lbrace> Q \<rbrace>"
   apply (drule shortest_path_exists)
   apply clarsimp
-  apply (rename_tac l)
-  apply (case_tac l rule: remdups_adj.cases)
-    apply clarsimp
-   apply clarsimp
-  apply (rule bexI[rotated])
-   apply clarsimp
-   apply assumption
+  apply (rename_tac xs)
+  apply (case_tac xs rule: remdups_adj.cases; clarsimp)
+  apply (rename_tac r' s' ys)
+  apply (case_tac s', clarsimp)
+  apply (rule bexI[rotated], assumption)
   apply clarify
-  apply (simp only: valid_path.simps, clarify)
   apply (frule shortest_path_is_shortest [where Q=Q])
    apply simp
   apply clarsimp
   apply (drule valid_path_implies_exs_valid_whileLoop)
   apply (clarsimp simp: exs_valid_def)
   apply (erule bexI [rotated])
-  apply (clarsimp split: if_split_asm)
+  apply (clarsimp split: if_split_asm simp: split_pairs)
   done
 
 lemma exs_valid_whileLoop_complete:
-   "(\<exists>T R.
-         (\<forall>s. P s \<longrightarrow> T r s)
-         \<and> (\<forall>r s0. \<lbrace> \<lambda>s. T r s \<and> C r s \<and> s = s0 \<rbrace> B r
-                            \<exists>\<lbrace> \<lambda>r' s'. T r' s' \<and> ((r', s'), (r, s0)) \<in> R \<rbrace>)
-         \<and> wf R
-         \<and> (\<forall>r s. (T r s \<and> \<not> C r s) \<longrightarrow> Q r s))
-      = (\<lbrace> P \<rbrace> whileLoop C B r \<exists>\<lbrace> Q \<rbrace>)"
+  "(\<exists>T R. (\<forall>s. P s \<longrightarrow> T r s)
+          \<and> (\<forall>r s0. \<lbrace> \<lambda>s. T r s \<and> C r s \<and> s = s0 \<rbrace>
+                    B r
+                    \<exists>\<lbrace> \<lambda>r' s'. T r' s' \<and> ((r', s'), (r, s0)) \<in> R \<rbrace>)
+          \<and> wf R
+          \<and> (\<forall>r s. (T r s \<and> \<not> C r s) \<longrightarrow> Q r s))
+   = (\<lbrace> P \<rbrace> whileLoop C B r \<exists>\<lbrace> Q \<rbrace>)"
   (is "(\<exists>T R. ?LHS T R) = ?RHS")
 proof (rule iffI)
   assume lhs: "\<exists>T R. ?LHS T R"
@@ -384,15 +376,15 @@ next
   assume rhs: "?RHS"
 
   define I where "I \<equiv> \<lambda>r s. \<lbrace> \<lambda>s'. s' = s \<rbrace> whileLoop C B r \<exists>\<lbrace> Q \<rbrace>"
-
   define R where "R \<equiv> measure (\<lambda>(r, s). shortest_path_length C B (r, s) Q)"
 
   have P_s: "\<And>s. P s \<Longrightarrow> I r s"
     using rhs
     by (clarsimp simp: I_def exs_valid_def)
 
-  have inv_holds: "\<And>r s. \<lbrakk> I r s; C r s \<rbrakk> \<Longrightarrow>
-              \<exists>(r', s') \<in> fst (B r s). I r' s' \<and> ((r', s'), r, s) \<in> R"
+  have inv_holds:
+  "\<And>r s. \<lbrakk> I r s; C r s \<rbrakk> \<Longrightarrow> \<exists>(r', s') \<in> fst (B r s). I r' (with_env_of s s') \<and>
+                                                       ((r', (with_env_of s s')), r, s) \<in> R"
     apply (clarsimp simp: I_def R_def)
     apply (frule (1) shortest_path_gets_shorter)
     apply clarsimp
@@ -404,16 +396,13 @@ next
     by (clarsimp simp: R_def)
 
   have last_step: "\<And>r s. \<lbrakk> I r s; \<not> C r s \<rbrakk> \<Longrightarrow> Q r s"
-    apply (clarsimp simp: I_def exs_valid_def)
-    apply (metis in_return whileLoop_cond_fail)
-    done
+    unfolding I_def exs_valid_def
+    by clarsimp (metis fst_whileLoop_cond_false whileLoop_cond_fail)
 
   show "\<exists>I R. ?LHS I R"
-    apply (rule exI [where x=I])
-    apply (rule exI [where x=R])
     using P_s inv_holds wf_R last_step
-    apply (clarsimp simp: exs_valid_def)
-    done
+    unfolding exs_valid_def
+    by (smt (verit, ccfv_threshold) case_prodD case_prodI2)
 qed
 
 end
