lib/Monads/nondet/Nondet_Env.thy
@@ -1,0 +1,65 @@
+(*
+ * Copyright 2025, Proofcraft Pty Ltd
+ *
+ * SPDX-License-Identifier: BSD-2-Clause
+ *)
+
+theory Nondet_Env
+  imports Nondet_Monad
+begin
+
+subsection \<open>Basic properties about the Environment State\<close>
+
+(* When the reader state is unit, the `mstate` field is the only relevant information *)
+lemmas mstate_cong = arg_cong[where f=mstate]
+lemmas mstate_cong_unit = mstate_cong[where 'a=unit]
+
+lemma monad_state_unit_collapse[simp]:
+  "monad_state () (mstate s) = s"
+  by (cases s) simp
+
+lemma eq_with_env_of_mstate[simp]:
+  "(s = with_env_of s s') = (mstate s = s')"
+  by (cases s, auto)
+
+lemma with_env_of_eq_mstate: (* not simp, can lead to non-termination *)
+  "(with_env_of s s' = s) = (mstate s = s')"
+  by (cases s, auto)
+
+lemma mstate_map_state[simp]:
+  "mstate (map_state f s) = f (mstate s)"
+  by (simp add: map_state_def)
+
+lemma env_map_state[simp]:
+  "env (map_state f s) = env s"
+  by (simp add: map_state_def)
+
+lemma map_state_monad_state[simp]:
+  "map_state f (monad_state c s) = monad_state c (f s)"
+  by (simp add: map_state_def)
+
+lemma mstate_const_env[simp]:
+  "mstate (const_env f s) = mstate (f s)"
+  by (simp add: const_env_def)
+
+lemma env_const_env[simp]:
+  "env (const_env f s) = env s"
+  by (simp add: const_env_def)
+
+lemma const_env_monad_state[simp]:
+  "const_env f (monad_state c s) = monad_state c (mstate (f (monad_state c s)))"
+  by (simp add: map_state_def)
+
+lemma const_env_idem[simp]:
+  "const_env (const_env f) = const_env f"
+  by (simp add: const_env_def)
+
+lemma is_const_env_const_env:
+  "is_const_env (const_env f)"
+  by (simp add: is_const_env_def)
+
+lemma is_const_env_id:
+  "is_const_env f \<Longrightarrow> const_env f = f"
+  by (auto simp: is_const_env_def const_env_def)
+
+end
