lib/Monads/nondet/Nondet_Reader_Option.thy
@@ -23,7 +23,7 @@ translations
   "_doO (_nobind b) e"     == "b |>> (CONST K_bind e)"
   "DO x <- a; e OD"        == "a |>> (\<lambda>x. e)"
 
-
+(* These are here, because K_bind is not available yet in  Reader_Option_VCG *)
 lemma ovalid_K_bind_wp[wp]:
   "ovalid P f Q \<Longrightarrow> ovalid P (K_bind f x) Q"
   by simp
@@ -36,8 +36,15 @@ lemma no_ofail_K_bind[wp]:
   "no_ofail P f \<Longrightarrow> no_ofail P (K_bind f x)"
   by simp
 
+(* The connection between the reader option monad and the nondet monad is the nondet operator
+   "gets_the". We generally want the environment state of the nondet monad to be available to
+   the reader option monad, since the reader monad may want to make decisions that depend on
+   the environment state. Because gets_the is constructed via gets, it has the whole monad
+   state available, including the environment part. This makes it possible to use the same P
+   in the following rule for the reader option monad and the nondet monad, without any type
+   lifting. *)
 lemma no_ofail_gets_the_eq:
-  "no_ofail P f \<longleftrightarrow> no_fail P (gets_the (f :: ('s, 'a) lookup))"
+  "no_ofail P f \<longleftrightarrow> no_fail P (gets_the f)"
   by (auto simp: no_ofail_def no_fail_def gets_the_def gets_def
                  get_def assert_opt_def bind_def return_def fail_def
          split: option.split)
@@ -46,7 +53,10 @@ lemmas no_ofail_gets_the =
   no_ofail_gets_the_eq[THEN iffD1]
 
 
-(* Lemmas relating ovalid and valid *)
+(* Lemmas relating ovalid and valid. See comment above for no_ofail_gets_the_eq -- we can use
+   P and Q with the same type here, because of our choice of type for get/gets/get_the.
+   Similarly, the gets_the f rewrites below are possible to write nicely because the types
+   coincide. *)
 lemma ovalid_gets_the:
   "ovalid P f Q \<Longrightarrow> \<lbrace>P\<rbrace> gets_the f \<lbrace>Q\<rbrace>"
   apply wpsimp
@@ -129,7 +139,7 @@ lemma gets_obind_bind_eq:
   by (auto simp: simpler_gets_def bind_def obind_def return_def split: option.splits)
 
 lemma fst_assert_opt:
-  "fst (assert_opt opt s) = (if opt = None then {} else {(the opt,s)})"
+  "fst (assert_opt opt s) = (if opt = None then {} else {(the opt, mstate s)})"
   by (clarsimp simp: assert_opt_def fail_def return_def split: option.split)
 
 
@@ -145,65 +155,87 @@ section "Relation between option monad loops and non-deterministic monad loops."
 (* Option monad whileLoop formalisation thanks to Lars Noschinski <noschinl@in.tum.de>. *)
 
 lemma gets_the_conv:
-  "(gets_the B s) = (case B s of Some r' \<Rightarrow> ({(r', s)}, False) | _ \<Rightarrow> ({}, True))"
-  by (auto simp: gets_the_def gets_def get_def bind_def return_def fail_def assert_opt_def split: option.splits)
+  "(gets_the B s) = (case B s of Some r' \<Rightarrow> ({(r', mstate s)}, False) | _ \<Rightarrow> ({}, True))"
+  by (auto simp: gets_the_def gets_def get_def bind_def return_def fail_def assert_opt_def
+           split: option.splits)
 
 lemma gets_the_loop_terminates:
-  "whileLoop_terminates C (\<lambda>a. gets_the (B a)) r s
-    \<longleftrightarrow> (\<exists>rs'. (Some r, rs') \<in> option_while' (\<lambda>a. C a s) (\<lambda>a. B a s))" (is "?L \<longleftrightarrow> ?R")
+  "whileLoop_terminates C (\<lambda>a. gets_the (B a)) c r s
+    \<longleftrightarrow> (\<exists>rs'. (Some r, rs') \<in> option_while' (\<lambda>a. C a (monad_state c s)) (\<lambda>a. B a (monad_state c s)))" (is "?L \<longleftrightarrow> ?R")
 proof
   assume ?L then show ?R
   proof (induct rule: whileLoop_terminates.induct[case_names 1 2])
     case (2 r s) then show ?case
-      by (cases "B r s") (auto simp: gets_the_conv intro: option_while'.intros)
+      by (cases "B r (monad_state c s)") (auto simp: gets_the_conv intro: option_while'.intros)
   qed (auto intro: option_while'.intros)
 next
   assume ?R then show ?L
   proof (elim exE)
-    fix rs' assume "(Some r, rs') \<in> option_while' (\<lambda>a. C a s) (\<lambda>a. B a s)"
-    then have "whileLoop_terminates C (\<lambda>a. gets_the (B a)) (the (Some r)) s"
+    fix rs' assume "(Some r, rs') \<in> option_while' (\<lambda>a. C a (monad_state c s)) (\<lambda>a. B a (monad_state c s))"
+    then have "whileLoop_terminates C (\<lambda>a. gets_the (B a)) c (the (Some r)) s"
       by induct (auto intro: whileLoop_terminates.intros simp: gets_the_conv)
     then show ?thesis by simp
   qed
 qed
 
 lemma gets_the_whileLoop:
-  fixes C :: "'a \<Rightarrow> 's \<Rightarrow> bool"
-  shows "whileLoop C (\<lambda>a. gets_the (B a)) r = gets_the (owhile C B r)"
+  "whileLoop C (\<lambda>a. gets_the (B a)) r = gets_the (owhile C B r)"
 proof -
-  { fix r s r' s' assume "(Some (r,s), Some (r', s')) \<in> whileLoop_results C (\<lambda>a. gets_the (B a))"
-    then have "s = s' \<and> (Some r, Some r') \<in> option_while' (\<lambda>a. C a s) (\<lambda>a. B a s)"
+  {
+    fix r s r' s' c
+    assume "(Some (r,s), Some (r', s')) \<in> whileLoop_results C (\<lambda>a. gets_the (B a)) c"
+    then
+    have "s = s' \<and>
+          (Some r, Some r') \<in> option_while' (\<lambda>a. C a (monad_state c s)) (\<lambda>a. B a (monad_state c s))"
     by (induct "Some (r, s)" "Some (r', s')" arbitrary: r s)
-       (auto intro: option_while'.intros simp: gets_the_conv split: option.splits) }
+       (auto intro: option_while'.intros simp: gets_the_conv split: option.splits)
+  }
   note wl'_Inl = this
 
-  { fix r s assume "(Some (r,s), None) \<in> whileLoop_results C (\<lambda>a. gets_the (B a))"
-    then have "(Some r, None) \<in> option_while' (\<lambda>a. C a s) (\<lambda>a. B a s)"
-      by (induct "Some (r, s)" "None :: (('a \<times> 's) option)" arbitrary: r s)
-         (auto intro: option_while'.intros simp: gets_the_conv split: option.splits) }
+  {
+    fix r s c
+    assume "(Some (r,s), None) \<in> whileLoop_results C (\<lambda>a. gets_the (B a)) c"
+    then
+    have "(Some r, None) \<in> option_while' (\<lambda>a. C a (monad_state c s)) (\<lambda>a. B a (monad_state c s))"
+      by (induct "Some (r, s)" "None :: (('c \<times> 'b) option)" arbitrary: r s)
+         (auto intro: option_while'.intros simp: gets_the_conv split: option.splits)
+  }
   note wl'_Inr = this
 
-  { fix r s r' assume "(Some r, Some r') \<in> option_while' (\<lambda>a. C a s) (\<lambda>a. B a s)"
-    then have "(Some (r,s), Some (r',s)) \<in> whileLoop_results C (\<lambda>a. gets_the (B a))"
+  {
+    fix r s r' c
+    assume "(Some r, Some r') \<in> option_while' (\<lambda>a. C a (monad_state c s)) (\<lambda>a. B a (monad_state c s))"
+    then
+    have "(Some (r,s), Some (r',s)) \<in> whileLoop_results C (\<lambda>a. gets_the (B a)) c"
     by (induct "Some r" "Some r'" arbitrary: r)
-       (auto intro: whileLoop_results.intros simp: gets_the_conv) }
+       (auto intro: whileLoop_results.intros simp: gets_the_conv)
+  }
   note option_while'_Some = this
 
-  { fix r s assume "(Some r, None) \<in> option_while' (\<lambda>a. C a s) (\<lambda>a. B a s)"
-    then have "(Some (r,s), None) \<in> whileLoop_results C (\<lambda>a. gets_the (B a))"
-    by (induct "Some r" "None :: 'a option" arbitrary: r)
-       (auto intro: whileLoop_results.intros simp: gets_the_conv) }
+  {
+    fix r s c
+    assume "(Some r, None) \<in> option_while' (\<lambda>a. C a (monad_state c s)) (\<lambda>a. B a (monad_state c s))"
+    then have "(Some (r,s), None) \<in> whileLoop_results C (\<lambda>a. gets_the (B a)) c"
+    by (induct "Some r" "None :: 'c option" arbitrary: r)
+       (auto intro: whileLoop_results.intros simp: gets_the_conv)
+  }
   note option_while'_None = this
 
-  have "\<And>s. owhile C B r s = None
-          \<Longrightarrow> whileLoop C (\<lambda>a. gets_the (B a)) r s = ({}, True)"
-    by (auto simp: whileLoop_def owhile_def option_while_def option_while'_THE gets_the_loop_terminates
-      split: if_split_asm dest: option_while'_None wl'_Inl option_while'_inj)
+  have "\<And>s. owhile C B r s = None \<Longrightarrow> whileLoop C (\<lambda>a. gets_the (B a)) r s = ({}, True)"
+    unfolding whileLoop_def owhile_def option_while_def
+    by (fastforce simp: option_while'_THE gets_the_loop_terminates option_while'_None
+                  split: if_split_asm
+                  dest!: wl'_Inl
+                  dest: option_while'_inj)
   moreover
   have "\<And>s r'. owhile C B r s = Some r'
-          \<Longrightarrow> whileLoop C (\<lambda>a. gets_the (B a)) r s = ({(r', s)}, False)"
-    by (auto simp: whileLoop_def owhile_def option_while_def option_while'_THE gets_the_loop_terminates
-      split: if_split_asm dest: wl'_Inl wl'_Inr option_while'_inj intro: option_while'_Some)
+                \<Longrightarrow> whileLoop C (\<lambda>a. gets_the (B a)) r s = ({(r', mstate s)}, False)"
+    unfolding whileLoop_def owhile_def option_while_def
+    by (fastforce simp: option_while'_THE gets_the_loop_terminates option_while'_None
+                  split: if_split_asm
+                  dest!: wl'_Inr  wl'_Inl
+                  dest: option_while'_inj
+                  intro: option_while'_Some)
   ultimately
   show ?thesis
     by (auto simp: fun_eq_iff gets_the_conv split: option.split)
